Prove interpretation refinement based on specs
Fairly significant re-structuring and cleanup. There is now only one
interpretation statement, which says that rexec of the implementation
with the fixed, layer recovery procedure implies (trace inclusion) crash
execution of the spec layer. This theorem is proven using recovery
specifications for each operation that gives normal execution
correctness and crash-recovery idempotence.

src/Shallow/Interpret.v
@@ -1,5 +1,7 @@
 Require Import ProgLang.Prog.
 Require Import ProgLang.ProgTheorems.
+Require Import ProgLang.Hoare.
+Require Import ProgLang.HoareRecovery.
 Require Import Automation.
 
 (* Language 1 is the implementation, language 2 is the spec:
@@ -13,6 +15,16 @@ Section Interpreter.
   Notation prog2 := (prog opT2).
 
   Variable op_impl: forall T, opT2 T -> prog1 T.
+  (* for now, recovery must make all changes to state and cannot preserve
+     its return value
+
+     TODO: for log, need to generalize this or have recovery store result in
+     variable
+
+     TODO: might want to allow recovery to return an error code and make no
+     promises
+   *)
+  Variable rec: prog1 unit.
 
   Fixpoint interpret T (p: prog2 T) : prog1 T :=
     match p with
@@ -26,8 +38,54 @@ Section Interpreter.
   Variable step2: Semantics opT2 State2.
 
   Variable invariant: State1 -> Prop.
-  Variable crash_invariant: State1 -> Prop.
   Variable abstraction: State1 -> State2.
+
+  Hypothesis
+    (Hop_recover_ok: forall T (op:opT2 T),
+        prog_rspec
+          (fun (_:unit) state =>
+             {|
+               rec_pre := invariant state;
+               rec_post :=
+                 fun v state' => invariant state' /\
+                          step2 op (abstraction state) v (abstraction state');
+               recover_post :=
+                 fun _ state' =>
+                   invariant state' /\
+                   (abstraction state' = abstraction state \/
+                    exists v, step2 op (abstraction state) v (abstraction state'));
+             |})
+          (op_impl op)
+          rec
+          step1).
+
+  (* This condition is required for two reasons:
+
+   - there might be no operations, and recovery still has to work in that case
+   - when we crash while running pure code, the recovery procedure really needs
+     to not do anything to the abstraction
+
+     The condition is fairly trivial because it almost follows from the recovery
+     specs in Hop_recover_ok; in particular, it would actually follow from
+     prog_rspec of any read-only operation. Unfortunately there's no guarantee
+     there are any read-only operations; in practice, this theorem is likely to
+     be a lemma for the recovery procedure in a realistic prog layer.
+   *)
+  Hypothesis
+    (Hret_recover:
+       prog_loopspec
+         (fun (_:unit) state =>
+            {|
+              pre := invariant state;
+              post :=
+                fun v state' => invariant state' /\
+                         abstraction state' = abstraction state;
+              crash :=
+                fun state' => invariant state' /\
+                       abstraction state' = abstraction state;
+            |})
+         rec
+         step1).
 
   Notation exec1 := (exec step1).
   Notation exec2 := (exec step2).
@@ -36,196 +94,82 @@ Section Interpreter.
 
   Set Default Proof Using "All".
 
-  (* TODO: in general, it might not be the case that crash states line up with
-  abstract states as desired; there might be states that are only exposed by
-  recovery and that are then patched up during recovery. *)
-  Definition res_abstraction T (r: Result State1 T) : Result State2 T :=
+  Definition res_abstraction T (r: RResult State1 T unit) : Result State2 T :=
     match r with
-    | Finished v state => Finished v (abstraction state)
-    | Crashed state => Crashed (abstraction state)
+    | RFinished v state => Finished v (abstraction state)
+    | Recovered _ state => Crashed (abstraction state)
     end.
 
-  Definition res_invariant T (r: Result State1 T) : Prop :=
+  Definition res_invariant T R (r: RResult State1 T R) : Prop :=
     match r with
-    | Finished _ state => invariant state
-    | Crashed state => crash_invariant state
+    | RFinished _ state => invariant state
+    | Recovered _ state => invariant state
     end.
+
+  Theorem rexec_impl : forall T (op:opT2 T) state r,
+      invariant state ->
+      rexec1 (op_impl op) rec state r ->
+      match r with
+      | RFinished v state' =>
+        invariant state' /\
+        step2 op (abstraction state) v (abstraction state')
+      | Recovered _ state' =>
+        invariant state' /\
+        (abstraction state' = abstraction state \/
+         exists v, step2 op (abstraction state) v (abstraction state'))
+      end.
+  Proof.
+    intros.
+    eapply Hop_recover_ok in H0; simpl in *; intuition.
+  Qed.
 
   (* TODO: this property shouldn't be called interpretation, need a more
   intuitive name *)
   Definition interpretation :=
     forall T (p: prog2 T) state r,
       invariant state ->
-      exec1 (interpret p) state r ->
+      (* TODO: is this the right phrasing? will it chain between layers
+      correctly?
+
+       It does have the advantage of being somewhat minimal: the implementation
+       + recovery will implement the crash behavior of the upper layer, which
+       implies something about running with rec >> interpret r hopefully. *)
+      rexec1 (interpret p) rec state r ->
       exec2 p (abstraction state) (res_abstraction r) /\
       res_invariant r.
 
   Hint Constructors exec.
 
-  Hypothesis (Hcrash_invariant: forall state, invariant state -> crash_invariant state).
-
-  Theorem interpret_exec :
-    (* every operation is implemented according to the step semantics of the
-    spec language *)
-    forall (Hop_ok: forall T (op: opT2 T) state v state',
-          invariant state ->
-          exec1 (op_impl op) state (Finished v state') ->
-          step2 op (abstraction state) v (abstraction state') /\ invariant state')
-      (* every implementation crashes in states that are abstractly either the
-        pre state or the post state *)
-      (Hop_crash: forall T (op: opT2 T) state state',
-          invariant state ->
-          exec1 (op_impl op) state (Crashed state') ->
-          (abstraction state' = abstraction state \/
-           exists v, step2 op (abstraction state) v (abstraction state')) /\
-          crash_invariant state'),
-      interpretation.
+  Theorem interpret_exec : interpretation.
   Proof.
     unfold interpretation.
     induction p; simpl; intros.
-    - destruct r; simpl.
-      + eapply Hop_ok in H0; eauto.
-        intuition eauto.
-      + eapply Hop_crash in H0; intuition eauto;
-          repeat deex;
-          eauto.
+    - eapply rexec_impl in H0; eauto.
+      destruct r; simpl; intuition eauto.
+      replace (abstraction state0); eauto.
+      deex; eauto.
+    - apply rexec_ret in H0.
+      destruct r.
+      + simpl; intuition (subst; eauto).
+      + eapply Hret_recover in H0; simpl in *; safe_intuition; auto.
         replace (abstraction state0); eauto.
-    - inv_exec; simpl; eauto.
-    - inv_exec.
-      + match goal with
+    - inversion H1; subst; simpl.
+      + inv_exec.
+        match goal with
         | [ Hexec: exec1 (interpret p) _ _ |- _ ] =>
-          eapply IHp in Hexec; simpl in *; eauto; safe_intuition
+          eapply RExec in Hexec;
+            eapply IHp in Hexec; eauto; safe_intuition
         end.
         match goal with
         | [ Hexec: exec1 (interpret (p0 _)) _ _ |- _ ] =>
-          eapply H in Hexec; eauto; safe_intuition
+          eapply RExec in Hexec;
+            eapply H in Hexec; eauto; safe_intuition
         end.
         intuition eauto.
-      + match goal with
-        | [ Hexec: exec1 (interpret p) _ _ |- _ ] =>
-          eapply IHp in Hexec; simpl in *; eauto; safe_intuition
-        end.
-        intuition eauto.
-  Qed.
-
-  Definition rres_abstraction T R (r: RResult State1 T R) : RResult State2 T R :=
-    match r with
-    | RFinished v state => RFinished v (abstraction state)
-    | Recovered v state => Recovered v (abstraction state)
-    end.
-
-  Definition rres_invariant T R (r: RResult State1 T R) : Prop :=
-    match r with
-    | RFinished _ state => invariant state
-    | Recovered _ state => invariant state
-    end.
-
-  (* for now, recovery must make all changes to state and cannot preserve
-     its return value
-
-     TODO: for log, need to generalize this or have recovery store result in
-     variable *)
-  Variable rec: prog1 unit.
-
-  Definition exec_recover_interpretation :=
-    forall R (pr: prog2 R) state rv state',
-      crash_invariant state ->
-      exec_recover step1 (Bind rec (fun _ => interpret pr)) state rv state' ->
-      exec_recover step2 pr (abstraction state) rv (abstraction state') /\
-      invariant state'.
-
-  Definition rexec_interpretation :=
-    forall T (p: prog2 T) R (pr: prog2 R) state r,
-      invariant state ->
-      rexec1 (interpret p) (Bind rec (fun _ => interpret pr)) state r ->
-      rexec2 p pr (abstraction state) (rres_abstraction r) /\
-      rres_invariant r.
-
-  Hypothesis (Hinterp: interpretation).
-
-  Hypothesis
-      (Hrec: forall state r, exec step1 rec state r ->
-                    crash_invariant state ->
-                    res_invariant r /\
-                    match r with
-                    | Finished _ state' =>
-                      (* TODO: too strong - what the recovery procedure needs to
-                         guarantee is that it preserves the crash abstractions
-                         of [interpret p] (that is, when [state] is a crash state of
-                         [interpret p], the recovery can produce [state'] with an
-                         abstraction)
-
-                         Note that this can be phrased as a per-operation
-                         assumption that implies a property about all
-                         interpreted programs. *)
-                      abstraction state' = abstraction state
-                    | Crashed state' =>
-                      (* TODO: in this case, similar to Finished case we will
-                      guarantee the abstraction is from some crash state *)
-                      abstraction state' = abstraction state
-                    end).
-
-  Ltac cleanup := simpl in *; eauto; safe_intuition;
-                  try match goal with
-                      | |- _ /\ _ =>
-                        split; [ | solve [ eauto ]]
-                      end.
-
-  Hint Constructors exec_recover.
-
-  Ltac forward_specs :=
-    repeat match goal with
-           | [ H: exec _ rec _ _ |- _ ] =>
-             eapply Hrec in H; cleanup
-           | [ H: exec _ (interpret _) _ _ |- _ ] =>
-             eapply Hinterp in H; cleanup
-           end;
-    repeat match goal with
-             (* TODO: this will have to be more sophisticated with proper
-             recovery crash correctness handling *)
-           | [ H: abstraction _ = abstraction _ |- _ ] =>
-             rewrite H in *
-           end;
-    eauto.
-
-  Theorem interpret_exec_recover : exec_recover_interpretation.
-  Proof.
-    unfold interpretation, exec_recover_interpretation; intros.
-    induction H0.
-    - inv_exec; forward_specs.
-    - inv_exec; forward_specs.
-  Qed.
-
-  Hint Constructors rexec.
-
-  Theorem interpret_rexec : rexec_interpretation.
-  Proof.
-    unfold interpretation, rexec_interpretation; intros.
-    match goal with
-    | [ H: rexec _ _ _ _ _ |- _ ] =>
-      inversion H; subst; repeat sigT_eq
-    end.
-    - simpl; forward_specs.
-    - simpl; forward_specs.
-      eapply interpret_exec_recover in H2; cleanup.
-      eauto.
+      + eapply rexec_recover_bind_inv in H1; hyp_intuition; repeat deex.
+        eapply IHp in H1; safe_intuition; eauto.
+        eapply IHp in H1; safe_intuition; eauto.
+        eapply H in H4; safe_intuition; eauto.
   Qed.
 
 End Interpreter.
-
-Theorem interpretation_weaken : forall `(step1: Semantics opT1 State1)
-                                  `(step2: Semantics opT2 State2)
-                                  (step2': Semantics opT2 State2)
-                                  op_impl
-                                  invariant crash_invariant
-                                  abstraction,
-    semantics_impl step2 step2' ->
-    interpretation op_impl step1 step2 invariant crash_invariant abstraction ->
-    interpretation op_impl step1 step2' invariant crash_invariant abstraction.
-Proof.
-  unfold interpretation; intros.
-  intuition.
-  eapply exec_weaken; eauto.
-  eapply H0; eauto.
-  eapply H0; eauto.
-Qed.
